proof is getting there

src/Dmajortodflatmajor.v
@@ -39,10 +39,15 @@ Definition total_inj (mi : meminj) (m : mem) : Prop :=
       mi b = Some (b',0).
 
 (* Injection only deals with meaningful blocks *)
-Definition minimal_inj (mi : meminj) (m : mem) : Prop :=
+Definition minimal_inj_domain (mi : meminj) (m : mem) : Prop :=
   forall b x,
     mi b = Some x ->
     Mem.valid_block m b.
+
+Definition minimal_inj_range (mi : meminj) (m : mem) : Prop :=
+  forall b b' delta,
+    mi b = Some (b',delta) ->
+    Mem.valid_block m b'.
 
 (* local variables follow our injection *)
 Definition env_inj (mi : meminj) (e e' : env) : Prop :=
@@ -77,8 +82,8 @@ Definition wf_inj (mi : meminj) : Prop :=
   meminj_injective mi /\
   same_offsets mi.
 
-Definition wf_mem (mi : meminj) (m : mem) : Prop :=
-  wf_inj mi /\ total_inj mi m /\ minimal_inj mi m.
+Definition wf_mem (mi : meminj) (m : mem) (m' : mem) : Prop :=
+  wf_inj mi /\ total_inj mi m /\ minimal_inj_domain mi m /\ minimal_inj_range mi m'.
 
 Lemma free_stack_frame_mem_inj :
   forall mi m m' b sz,
@@ -210,7 +215,7 @@ Lemma eval_expr_transf :
     Dmajor.eval_expr ge e m exp v ->
     forall m' mi e' sp,
       Mem.inject mi m m' ->
-      wf_mem mi m ->
+      wf_mem mi m m' ->
       env_inj mi e e' ->
       exists v',
         eval_expr ge e' m' sp exp v' /\ Val.inject mi v v'.
@@ -228,7 +233,7 @@ Lemma eval_exprlist_transf :
     Dmajor.eval_exprlist ge e m l vl ->
     forall m' mi e' sp,
       Mem.inject mi m m' ->
-      wf_mem mi m ->
+      wf_mem mi m m' ->
       env_inj mi e e' ->
       exists vl',
         eval_exprlist ge e' m' sp l vl' /\ Val.inject_list mi vl vl'.
@@ -302,14 +307,14 @@ Inductive match_states : Dmajor.state -> Dflatmajor.state -> Prop :=
     Plt (highest_block k') b ->
     match_cont k k' mi m' ->
     env_inj mi e e' ->
-    wf_mem mi m ->
+    wf_mem mi m m' ->
     match_states
       (Dmajor.State f s k e m)
       (Dflatmajor.State f s k' (Vptr b Int.zero) e' m' z)
 | match_callstate : forall f args args' k k' m m' z mi,
     Mem.inject mi m m' ->
     match_cont k k' mi m' ->
-    wf_mem mi m ->
+    wf_mem mi m m' ->
     Val.inject_list mi args args' ->
     match_states
       (Dmajor.Callstate f args k m)
@@ -317,7 +322,7 @@ Inductive match_states : Dmajor.state -> Dflatmajor.state -> Prop :=
 | match_returnstate : forall v v' k k' m m' z mi,
     Mem.inject mi m m' ->
     match_cont k k' mi m' ->
-    wf_mem mi m ->
+    wf_mem mi m m' ->
     Val.inject mi v v' ->
     match_states
       (Dmajor.Returnstate v k m)
@@ -460,6 +465,7 @@ Lemma match_cont_alloc_store :
     forall lo hi m' b c v m'' b0,
       Mem.alloc m lo hi = (m',b) ->
       Mem.store c m' b lo v = Some m'' ->
+      mi b0 = None ->
       match_cont k k' (fun x => if peq x b0 then Some (b,0) else mi x) m''.
 Proof.
   induction 1; intros; try solve [econstructor; eauto].
@@ -468,11 +474,13 @@ Proof.
   eauto.
   unfold env_inj in *.
   intros.
-  eapply H0 in H6.
+  eapply H0 in H7.
   break_exists. break_and.
   eexists; split; eauto.
-  inv H7; econstructor; eauto.
-  admit. (* hmmm *)
+  invp (Val.inject mi v0 x); econstructor; eauto.
+  find_rewrite. break_match; eauto.
+  
+  subst. congruence.
 
   eauto.
 
@@ -495,33 +503,30 @@ Proof.
   clear H2. app H0 (Mem.load c0).
 Qed.
 
-Lemma minimal_inj_store :
+Lemma minimal_inj_domain_store :
   forall c m b ofs v m',
     Mem.store c m b ofs v = Some m' ->
     forall mi,
-      minimal_inj mi m ->
-      minimal_inj mi m'.
+      minimal_inj_domain mi m ->
+      minimal_inj_domain mi m'.
 Proof.
-  intros. unfold minimal_inj in *.
+  intros. unfold minimal_inj_domain in *.
   intros.
   unfold Mem.valid_block in *.
   erewrite Mem.nextblock_store; eauto.
 Qed.
 
-
-Lemma wf_mem_store :
-  forall mi m,
-    wf_mem mi m ->
-    forall c b ofs v m',
-      Mem.store c m b ofs v = Some m' ->
-      wf_mem mi m'.
+Lemma minimal_inj_range_store :
+  forall c m b ofs v m',
+    Mem.store c m b ofs v = Some m' ->
+    forall mi,
+      minimal_inj_range mi m ->
+      minimal_inj_range mi m'.
 Proof.
+  intros. unfold minimal_inj_range in *.
   intros.
-  unfold wf_mem in *.
-  break_and.
-  split. eauto.
-  split. eapply total_inj_store; eauto.
-  eapply minimal_inj_store; eauto.
+  unfold Mem.valid_block in *.
+  erewrite Mem.nextblock_store; eauto.
 Qed.
 
 
@@ -544,9 +549,410 @@ Proof.
   econstructor; eauto.
 Qed.
 
-Lemma wf_mem_store_mapped :
-  forall mi m,
+(* TODO: dedup this lemma *)
+(* TODO: version in Emajortodmajor is weaker *)
+Lemma alloc_store :
+  forall m lo hi m' b,
+    Mem.alloc m lo hi = (m',b) ->
+    forall v c,
+      hi - lo >= size_chunk c ->
+      (align_chunk c | lo) ->
+      { m'' : mem | Mem.store c m' b lo v = Some m''}.
+Proof.
+  intros.
+  app Mem.valid_access_alloc_same Mem.alloc; try omega.
+  app Mem.valid_access_implies Mem.valid_access.
+  2: instantiate (1 := Writable); econstructor; eauto.
+  eapply Mem.valid_access_store; eauto.
+Qed.
+
+(* TODO: dedup with above lemma *)
+Lemma store_align_inv :
+  forall c m0 lo hi m b v m',
+    Mem.alloc m0 lo hi = (m,b) ->
+    Mem.store c m b lo v = Some m' -> 
+    hi - lo >= size_chunk c /\ (align_chunk c | lo).
+Proof.
+  intros.
+  app Mem.store_valid_access_3 Mem.store.
+  unfold Mem.valid_access in *.
+  break_and.
+  split; eauto.
+  assert (hi - lo >= size_chunk c \/ hi - lo < size_chunk c) by omega.
+  destruct H3; eauto.
+
+  
+  assert (Mem.range_perm m b lo hi Cur Freeable).
+  unfold Mem.range_perm.
+  intros.
+  app Mem.perm_alloc_2 Mem.alloc.
+
+  unfold Mem.range_perm in H0.
+  remember (H0 lo) as Hlo.
+  remember (H0 (lo + size_chunk c - 1)) as Hc.
+  clear HeqHlo.
+  clear HeqHc.
+  clear H0.
+  assert (Hlop: Mem.perm m b lo Cur Writable).
+  eapply Hlo; destruct c; simpl; try omega.
+  clear Hlo.
+  
+  assert (Hcp: Mem.perm m b (lo + size_chunk c - 1) Cur Writable).
+  eapply Hc; destruct c; simpl; omega.
+  clear Hc. 
+
+  remember Mem.perm_alloc_3 as Hmp. clear HeqHmp.
+  specialize (Hmp _ _ _ _ _ H).
+  remember (Hmp _ _ _ Hlop) as Hlor.
+  remember (Hmp _ _ _ Hcp) as Hcpr.
+  omega.
+Qed.
+
+(* Non-shitty version of Mem library copy *)
+Theorem alloc_left_mapped_inject:
+  forall f m1 m2 lo hi m1' b1 b2 delta,
+  Mem.inject f m1 m2 ->
+  Mem.alloc m1 lo hi = (m1', b1) ->
+  Mem.valid_block m2 b2 ->
+  0 <= delta <= Int.max_unsigned ->
+  (forall ofs k p, Mem.perm m2 b2 ofs k p -> delta = 0 \/ 0 <= ofs < Int.max_unsigned) ->
+  (forall ofs k p, lo <= ofs < hi -> Mem.perm m2 b2 (ofs + delta) k p) ->
+  Mem.inj_offset_aligned delta (hi-lo) ->
+  (forall b delta' ofs k p,
+   f b = Some (b2, delta') ->
+   Mem.perm m1 b ofs k p ->
+   lo + delta <= ofs + delta' < hi + delta -> False) ->
+  let f' := fun b => if eq_block b b1 then Some(b2, delta) else f b in
+     Mem.inject f' m1' m2
+  /\ inject_incr f f'
+  /\ f' b1 = Some(b2, delta)
+  /\ (forall b, b <> b1 -> f' b = f b).
+Proof.
+  intros. inversion H.
+  assert (inject_incr f f').
+    red; unfold f'; intros. destruct (eq_block b b1). subst b.
+    assert (f b1 = None). eauto with mem. congruence.
+    auto.
+  assert (Mem.mem_inj f' m1 m2).
+    inversion mi_inj; constructor; eauto with mem.
+    unfold f'; intros. destruct (eq_block b0 b1).
+      inversion H8. subst b0 b3 delta0.
+      elim (Mem.fresh_block_alloc _ _ _ _ _ H0). eauto with mem.
+      eauto.
+    unfold f'; intros. destruct (eq_block b0 b1).
+      inversion H8. subst b0 b3 delta0.
+      elim (Mem.fresh_block_alloc _ _ _ _ _ H0).
+      eapply Mem.perm_valid_block with (ofs := ofs). apply H9. generalize (size_chunk_pos chunk); omega.
+      eauto.
+    unfold f'; intros. destruct (eq_block b0 b1).
+      inversion H8. subst b0 b3 delta0.
+      elim (Mem.fresh_block_alloc _ _ _ _ _ H0). eauto with mem.
+      apply memval_inject_incr with f; auto.
+  split. constructor.
+(* inj *)
+  eapply Mem.alloc_left_mapped_inj; eauto. unfold f'; apply dec_eq_true.
+(* freeblocks *)
+  unfold f'; intros. destruct (eq_block b b1). subst b.
+  elim H9. eauto with mem.
+  eauto with mem.
+(* mappedblocks *)
+  unfold f'; intros. destruct (eq_block b b1). congruence. eauto.
+(* overlap *)
+  unfold f'; red; intros.
+  exploit Mem.perm_alloc_inv. eauto. eexact H12. intros P1.
+  exploit Mem.perm_alloc_inv. eauto. eexact H13. intros P2.
+  destruct (eq_block b0 b1); destruct (eq_block b3 b1).
+  congruence.
+  inversion H10; subst b0 b1' delta1.
+    destruct (eq_block b2 b2'); auto. subst b2'. right; red; intros.
+    eapply H6; eauto. omega.
+  inversion H11; subst b3 b2' delta2.
+    destruct (eq_block b1' b2); auto. subst b1'. right; red; intros.
+    eapply H6; eauto. omega.
+  eauto.
+(* representable *)
+  unfold f'; intros.
+  destruct (eq_block b b1).
+   subst. injection H9; intros; subst b' delta0. destruct H10.
+    exploit Mem.perm_alloc_inv; eauto; rewrite dec_eq_true; intro.
+    exploit H3. apply H4 with (k := Max) (p := Nonempty); eauto.
+    generalize (Int.unsigned_range_2 ofs). omega.
+   exploit Mem.perm_alloc_inv; eauto; rewrite dec_eq_true; intro.
+   exploit H3. apply H4 with (k := Max) (p := Nonempty); eauto.
+   generalize (Int.unsigned_range_2 ofs). omega.
+  eapply mi_representable; try eassumption.
+  destruct H10; eauto using Mem.perm_alloc_4.
+(* incr *)
+  split. auto.
+(* image of b1 *)
+  split. unfold f'; apply dec_eq_true.
+(* image of others *)
+  intros. unfold f'; apply dec_eq_false; auto.
+Qed.
+
+(* non-shitty version of Mem library copy *)
+Theorem alloc_parallel_inject:
+  forall f m1 m2 lo1 hi1 m1' b1 lo2 hi2,
+  Mem.inject f m1 m2 ->
+  Mem.alloc m1 lo1 hi1 = (m1', b1) ->
+  lo2 <= lo1 -> hi1 <= hi2 ->
+  exists m2', exists b2,
+  let f' := fun b => if eq_block b b1 then Some(b2,0) else f b in
+  Mem.alloc m2 lo2 hi2 = (m2', b2)
+  /\ Mem.inject f' m1' m2'.
+Proof.
+  intros.
+  case_eq (Mem.alloc m2 lo2 hi2). intros m2' b2 ALLOC.
+  exploit alloc_left_mapped_inject.
+  eapply Mem.alloc_right_inject; eauto.
+  eauto.
+  instantiate (1 := b2). eauto with mem.
+  instantiate (1 := 0). unfold Int.max_unsigned. generalize Int.modulus_pos; omega.
+  auto.
+  intros. apply Mem.perm_implies with Freeable; auto with mem.
+  eapply Mem.perm_alloc_2; eauto. omega.
+  red; intros. apply Zdivide_0.
+  intros.
+
+  assert (Mem.valid_block m2 b2) by (eapply Mem.valid_block_inject_2; eauto).
+  apply (Mem.valid_not_valid_diff m2 b2 b2); eauto with mem.  
+  
+  intros [A [B [C D]]].
+  exists m2'; exists b2; auto.
+  
+Qed.
+
+
+  
+Lemma wf_mem_store :
+  forall mi m m0,
+    wf_mem mi m m0 ->
+    forall c b ofs v v' m' m0' b',
+      Mem.store c m b ofs v = Some m' ->
+      Mem.store c m0 b' ofs v' = Some m0' ->
+      Val.inject mi v v' ->
+      mi b = Some (b',0) ->
+      wf_mem mi m' m0'.
+Proof.
+  intros.
+  unfold wf_mem in *.
+  break_and.
+  split. eauto.
+  split. eapply total_inj_store; eauto.
+  split.
+  eapply minimal_inj_domain_store; eauto.
+  eapply minimal_inj_range_store; eauto.
+Qed.
+
+Lemma wf_mem_alloc_not_mapped :
+  forall mi m m',
+    wf_mem mi m m' ->
+    forall lo hi m0 b,
+      Mem.alloc m lo hi = (m0,b) ->
+      mi b = None.
+Proof.
+  intros.
+  unfold wf_mem in *.
+  break_and.
+  unfold minimal_inj_domain in *.
+  destruct (mi b) eqn:?; try congruence.
+  eapply H2 in Heqo.
+  unfold Mem.valid_block in *.
+  app Mem.alloc_result Mem.alloc.
+  subst b.
+  eapply Plt_ne in Heqo.
+  congruence.
+Qed.
+
+Lemma wf_mem_alloc_not_mapped_to :
+  forall mi m m',
+    wf_mem mi m m' ->
+    forall lo hi m0 b',
+      Mem.alloc m' lo hi = (m0,b') ->
+      forall b0 b delta, mi b = Some (b0,delta) -> b0 <> b'.
+Proof.
+  intros.
+  unfold wf_mem in *.
+  break_and.
+  unfold minimal_inj_range in *.
+  eapply H4 in H1.
+  assert (~Mem.valid_block m' b') by (eauto with mem).
+  eapply Mem.valid_not_valid_diff; eauto.
+Qed.
+  
+
+Lemma wf_mem_alloc :
+  forall mi m m',
+    wf_mem mi m m' ->
+    forall lo hi m0 m0' b b',
+      Mem.alloc m lo hi = (m0,b) ->
+      Mem.alloc m' lo hi = (m0',b') ->
+      wf_mem (fun x => if eq_block x b then Some (b',0) else mi x) m0 m0'.
+Proof.
+  intros.
+  app wf_mem_alloc_not_mapped wf_mem.
+  assert (forall b0 b delta, mi b = Some (b0,delta) -> b0 <> b').
+  eapply wf_mem_alloc_not_mapped_to; eauto.
+  unfold wf_mem in *.
+  unfold wf_inj in *.
+  break_and.
+  
+  repeat split.
+
+  (* globals_inj_same *)
+  unfold globals_inj_same in *.
+  intros. eapply H2 in H9.
+  break_if; congruence.
+
+  (* meminj_injective *)
+  unfold meminj_injective in *.
+  intros.
+  destruct (eq_block b1 b2); try congruence.
+  destruct (eq_block b1 b);
+    destruct (eq_block b2 b); try congruence;
+    match goal with
+    | [ H : Some _ = Some _ |- _ ] => inv H
+    | [ |- _ ] => idtac
+    end; subst;
+      try congruence.
+  eapply H3 in H10. congruence.
+  eapply H3 in H9. congruence.
+  eapply H7; eauto.
+
+  (* same_offsets *)
+  unfold same_offsets.
+  intros.
+  break_if; simpl; eauto; congruence.
+
+  (* total_inj *)
+  unfold total_inj in *.
+  intros.
+  destruct (eq_block b0 b). eauto.
+  eapply H4; eauto.
+  erewrite <- Mem.load_alloc_unchanged; eauto.
+  eauto with mem.
+
+  (* minimal_inj_domain *)
+  unfold minimal_inj_domain.
+  intros. break_if. inv H9. eauto with mem.
+  unfold minimal_inj_domain in *.
+  eapply Mem.valid_block_alloc;
+  eauto.
+
+  (* minimal_inj_range *)
+  unfold minimal_inj_range in *.
+  intros. break_if. inv H9. eauto with mem.
+  eauto with mem.
+  
+  Unshelve.
+  econstructor.
+Qed.
+
+
+Lemma alloc_store_inject :
+  forall m lo hi m' b c m'' v,
+    Mem.alloc m lo hi = (m',b) ->
+    Mem.store c m' b lo v = Some m'' ->
+    forall mi m0 v',
+      Mem.inject mi m m0 ->
+      Val.inject mi v v' ->
+      wf_mem mi m m0 ->
+      exists m0' b' m0'',
+      let mi' := (fun x => if peq x b then Some (b',0) else mi x) in
+        Mem.alloc m0 lo hi = (m0',b') /\
+        Mem.store c m0' b' lo v' = Some m0'' /\
+        Mem.inject mi' m'' m0'' /\
+        wf_mem mi' m'' m0''.
+Proof.
+  intros.
+
+  app alloc_parallel_inject Mem.inject;
+    try eapply Z.le_refl.
+  destruct H1.
+
+  eapply val_inject_incr with (f2 := (fun b0 : positive => if eq_block b0 b then Some (x0, 0) else mi b0)) in H2.
+
+  
+  app Mem.store_mapped_inject Mem.store;
+    try erewrite Z.add_0_r in *.
+
+  eexists. eexists. eexists. simpl.
+  do 3 (split; eauto).
+  eapply wf_mem_alloc in H3; try eapply H1; try eapply H.
+  eapply wf_mem_store; eauto.
+  simpl; break_if; congruence.
+  simpl; break_if; congruence.
+
+  app wf_mem_alloc_not_mapped wf_mem.
+  unfold inject_incr.
+
+  intros.
+  break_if; congruence. 
+  
+Qed.
+  
+
+(* 
+
+
+(* TODO: Decompose this into smaller lemmas *)
+
+
+
+
+Lemma alloc_stack_frame :
+  forall mi m m',
+    Mem.inject mi m m' ->
     wf_mem mi m ->
+    forall lo hi,
+    exists m0 b,
+      Mem.alloc m' lo hi = (m0,b) /\
+      Mem.inject mi m m0 /\
+      (lo = 0 -> stack_frame_wf b hi mi m0).
+Proof.
+  intros.
+  destruct (Mem.alloc m' lo hi) eqn:?.
+  eexists. eexists. split. eauto.
+  split.
+  eapply Mem.alloc_right_inject; eauto.
+  intros.
+  unfold stack_frame_wf. split. subst lo.
+  unfold Mem.range_perm.
+  intros.
+  eapply Mem.perm_alloc_2; eauto.
+  intros. unfold wf_mem in *.
+  intro.
+  break_and.
+  unfold minimal_inj in *.
+  app H4 (mi b').
+  unfold Mem.valid_block in *.
+  eapply H4 in H2.
+  SearchAbout Mem.alloc.
+  SearchAbout Mem.inject.
+
+*)
+
+
+Lemma wf_mem_free_right :
+  forall mi m m',
+    wf_mem mi m m' ->
+    forall b lo hi m0,
+      Mem.free m' b lo hi = Some m0 ->
+      wf_mem mi m m0.
+Proof.
+  intros.
+  unfold wf_mem in *.
+  break_and.
+  repeat (split; eauto).
+  unfold minimal_inj_range in *.
+  intros. eapply H3 in H4.
+  unfold Mem.valid_block in *.
+  erewrite Mem.nextblock_free; eauto.
+Qed.
+  
+Lemma wf_mem_store_mapped :
+  forall mi m m0,
+    wf_mem mi m m0 ->
     forall c b ofs v m',
       Mem.store c m b ofs v  = Some m' ->
       exists b',
@@ -560,27 +966,107 @@ Proof.
   break_and.
   unfold same_offsets in *.
   rewrite H1. repeat f_equal.
-  eapply H5; eauto.
+  eauto.
 Qed.
 
-(* TODO: Decompose this into smaller lemmas *)
-Lemma alloc_store_inject :
-  forall m lo hi m' b c m'' v,
-    Mem.alloc m lo hi = (m',b) ->
-    Mem.store c m' b lo v = Some m'' ->
-    forall mi m0 v',
-      Mem.inject mi m m0 ->
-      Val.inject mi v v' ->
-      wf_mem mi m ->
-      exists m0' b' m0'',
-      let mi' := (fun x => if peq x b then Some (b',0) else mi x) in
-        Mem.alloc m0 lo hi = (m0',b') /\
-        Mem.store c m0' b' lo v' = Some m0'' /\
-        Mem.inject mi' m'' m0'' /\
-        wf_mem mi' m''.
-Proof.
-Admitted.
 
+Lemma stack_frame_allocated :
+  forall m sz m' b mi,
+    Mem.alloc m 0 sz = (m',b) ->
+    (forall b' delta, mi b' <> Some (b,delta)) ->
+    stack_frame_wf b sz mi m'.
+Proof.
+  intros.
+  unfold stack_frame_wf.
+  split. unfold Mem.range_perm.
+  intros.
+  eauto with mem.
+  eauto.
+Qed.
+
+
+Lemma wf_mem_alloc_right :
+  forall mi m m',
+    wf_mem mi m m' ->
+    forall lo hi m0 b,
+      Mem.alloc m' lo hi = (m0,b) ->
+      wf_mem mi m m0.
+Proof.
+  intros.
+  
+  remember wf_mem_alloc_not_mapped_to as nm2.
+  clear Heqnm2.
+  specialize (nm2 _ _ _ H _ _ _ _ H0).
+  
+  unfold wf_mem in *.
+  break_and. repeat (split; eauto).
+
+  unfold minimal_inj_range in *.
+  intros.
+
+  app nm2 (mi b0).
+  app H3 (mi b0).
+  eauto with mem. (* gosh I love this *)
+  
+Qed.
+  
+
+Lemma alloc_stack_frame :
+  forall sz mi m m',
+    wf_mem mi m m' ->
+    Mem.inject mi m m' ->
+    exists m0 b,
+      Mem.alloc m' 0 sz = (m0,b) /\
+      wf_mem mi m m0 /\
+      Mem.inject mi m m0 /\
+      stack_frame_wf b sz mi m0.
+Proof.
+  intros.
+  destruct (Mem.alloc m' 0 sz) eqn:?.
+  eexists. eexists. split; eauto.
+  split.
+  eapply wf_mem_alloc_right; eauto.
+  split.
+  eapply Mem.alloc_right_inject; eauto.
+  eapply stack_frame_allocated; eauto.
+  intros. intro.
+  app wf_mem_alloc_not_mapped_to wf_mem.
+Qed.
+
+Lemma env_inj_set_params :
+  forall names,
+  forall mi l l',
+    Val.inject_list mi l l' ->
+    env_inj mi (set_params l names) (set_params l' names).
+Proof.
+  induction names; intros.
+  simpl; unfold env_inj; intros.
+  rewrite PTree.gempty in *. congruence.
+  inv H. simpl. eapply IHnames in H.
+  simpl; unfold env_inj; intros.
+  intros. destruct (peq a id). subst. rewrite PTree.gss in *. inv H0. eauto.
+  rewrite PTree.gso in * by congruence.
+  eapply H; eauto.
+  simpl; unfold env_inj; intros.
+  intros. destruct (peq a id). subst. rewrite PTree.gss in *. inv H2. eauto.
+  rewrite PTree.gso in * by congruence.
+  eapply IHnames; eauto.
+Qed.
+
+
+
+Lemma env_inj_set_locals :
+  forall l mi e e',
+    env_inj mi e e' ->
+    env_inj mi (set_locals l e) (set_locals l e').
+Proof.
+  induction l; intros.
+  simpl. eauto.
+  simpl. unfold env_inj.
+  intros. destruct (peq a id). subst. rewrite PTree.gss in *. inv H0. eauto.
+  rewrite PTree.gso in * by congruence.
+  eapply IHl; eauto.
+Qed.
 
 Lemma single_step_correct:
   forall S1 t S2, Dmajor.step ge S1 t S2 ->
@@ -604,7 +1090,7 @@ Proof.
     eexists; split; try eapply plus_one; econstructor; eauto.
     eapply is_call_cont_transf; eauto.
     eapply match_cont_free_stack_frame; eauto.
-      
+    eapply wf_mem_free_right; eauto.
   * eexists; split; try eapply plus_one; econstructor; eauto.
     eapply env_inj_set; eauto.
 
@@ -613,6 +1099,7 @@ Proof.
   * destruct vaddr; simpl in *; try congruence.
     instantiate (1 := (Vptr b Int.zero)) in H9.
     instantiate (1 := (Vptr b Int.zero)) in H7.
+    
     app wf_mem_store_mapped wf_mem.
     app Mem.store_mapped_inject Mem.inject; try solve [invp Mem.inject; eauto].
     invp (Val.inject mi (Vptr b0 i)).
@@ -628,7 +1115,9 @@ Proof.
     rewrite Int.add_zero. rewrite Z.add_0_r in *. eauto.
     eapply match_cont_store; eauto.
     eapply wf_mem_store; eauto.
-
+    rewrite Z.add_0_r in *.
+    assumption.
+    
   * eexists; split; try eapply plus_one; econstructor; eauto.
     destruct vfp; simpl in *; try congruence.
     unfold Genv.find_funct in *.
@@ -647,6 +1136,7 @@ Proof.
   * invp external_call.
     invp Val.inject.
     app alloc_store_inject Mem.store.
+    
     match goal with
     | [ H : let _ := _ in _ |- _ ] => destruct H
     end.
@@ -663,6 +1153,8 @@ Proof.
     admit. (* need to thread it through *)
     
     eapply match_cont_alloc_store; eauto.
+    eapply wf_mem_alloc_not_mapped; eauto.
+    
     
     (* just env_inj proof here *)
     {
@@ -689,25 +1181,22 @@ Proof.
 
       subst.
       match goal with
-      | [ H : wf_mem mi m, H2 : Mem.alloc m _ _ = _, H3 : mi _ = _ |- _ ] => clear -H H2 H3
+      | [ H : wf_mem mi m m', H2 : Mem.alloc m _ _ = _, H3 : mi _ = _ |- _ ] => clear -H H2 H3
       end.
       unfold wf_mem in *;
         unfold wf_inj in *;
         break_and.
-      unfold minimal_inj in *.
+      unfold minimal_inj_domain in *.
 
       app Mem.alloc_result Mem.alloc.
-      (* haha backtracking match *)
-      match goal with
-      | [ H : _, H2: mi b0 = _ |- _ ] => eapply H in H2; clear H
-      end.
+      eapply H1 in H19; clear H1.
 
       subst b0. unfold Mem.valid_block in *.
       app Plt_ne Plt.
       congruence.
     } 
 
-      * eexists; split; try eapply plus_one; econstructor; eauto.
+  * eexists; split; try eapply plus_one; econstructor; eauto.
     econstructor; eauto.
   * eexists; split; try eapply plus_one; econstructor; eauto.
     econstructor; eauto.
@@ -717,13 +1206,25 @@ Proof.
     eexists; split; try eapply plus_one; econstructor; eauto.
     eapply match_call_cont; eauto.
     eapply match_cont_free_stack_frame; eauto.
+    eapply wf_mem_free_right; eauto.
   * app free_stack_frame stack_frame_wf.
     eexists; split; try eapply plus_one; econstructor; eauto; try eapply match_call_cont; eauto.
     eapply match_cont_free_stack_frame; eauto.
-  * (* This is an interesting one *)
-    (* we have to allocate memory *)
-    (* but we don't have to stick it in the injection *)
+    eapply wf_mem_free_right; eauto.
+  * app (alloc_stack_frame (fn_stackspace f)) wf_mem.
+    eexists; split; try eapply plus_one; econstructor; eauto.
+
+    (* This one's annoying *)
     admit.
+
+    (* This needs some thinking *)
+    admit.
+
+
+    eapply env_inj_set_locals;
+    eapply env_inj_set_params; eauto.
+
+    
   * inv H2.
     eexists; split; try eapply plus_one; try econstructor; eauto.
     (* match_cont needs Kcall to contain a Vptr for sp *)
